Add functions and some notes on how to craft a nice interface

kremlib/LowStar.Lib.AssocList.fst
@@ -16,7 +16,7 @@ module LL1 = LowStar.Lib.LinkedList
 open FStar.HyperStack.ST
 open LowStar.BufferOps
 
-#set-options "--fuel 1 --ifuel 1"
+#set-options "--fuel 0 --ifuel 0"
 
 /// We prefer the packed representation that is in general easier to use and will
 /// look at the underlying predicate-based representation from LL1 only when
@@ -48,6 +48,18 @@ val invariant: #t_k:eqtype -> #t_v:Type0 -> h:HS.mem -> ll:t t_k t_v -> Type0
 let invariant #_ #_ h ll =
   LL2.invariant h ll
 
+val footprint: #t_k:eqtype -> #t_v:Type0 -> h:HS.mem -> ll:t t_k t_v -> Ghost B.loc
+  (requires invariant h ll)
+  (ensures fun _ -> True)
+let footprint #_ #_ h ll =
+  LL2.footprint h ll
+
+/// What's the best way for clients to reason about this? Maybe a lemma that says:
+///
+/// B.(loc_disjoint l (loc_all_regions_from true r)) ==> B.(loc_disjoint l (footprint h ll))
+///
+/// This would allow clients to deduce that their own allocations are disjoint from the footprint of this. And also to apply the framing lemma with proper patterns!
+
 /// Proper recursion can only be done over the LL1.t type (unpacked representation).
 val find_ (#t_k: eqtype) (#t_v: Type0) (hd: LL1.t (t_k & t_v)) (l: G.erased (list (t_k & t_v))) (k: t_k):
   Stack (option t_v)
@@ -59,6 +71,7 @@ val find_ (#t_k: eqtype) (#t_v: Type0) (hd: LL1.t (t_k & t_v)) (l: G.erased (lis
       h0 == h1 /\
       x == M.sel m k)
 
+#push-options "--fuel 1 --ifuel 1"
 let rec find_ #_ #_ hd l k =
   if B.is_null hd then
     None
@@ -68,6 +81,7 @@ let rec find_ #_ #_ hd l k =
       Some (snd cell.LL1.data)
     else
       find_ cell.LL1.next (List.Tot.tl l) k
+#pop-options
 
 /// A wrapper for LL2
 
@@ -82,3 +96,16 @@ val find (#t_k: eqtype) (#t_v: Type0) (ll: t t_k t_v) (k: t_k):
 
 let find #_ #_ ll k =
   find_ !*ll.LL2.ptr !*ll.LL2.v k
+
+val add (#t_k: eqtype) (#t_v: Type0) (ll: t t_k t_v) (k: t_k) (x: t_v):
+  ST unit
+    (requires fun h0 ->
+      invariant h0 ll)
+    (ensures fun h0 _ h1 ->
+      B.modifies (footprint h0 ll) h0 h1 /\
+      v h1 ll == M.upd (v h0 ll) k (Some x))
+
+#push-options "--fuel 1"
+let add #_ #_ ll k x =
+  LL2.push ll (k, x)
+#pop-options
